src/StandaloneOCamlMain.v
@@ -15,7 +15,6 @@ Global Unset Extraction Optimize.
 
 (** Work around COQBUG(https://github.com/coq/coq/issues/4875) / COQBUG(https://github.com/coq/coq/issues/7954) / COQBUG(https://github.com/coq/coq/issues/7954) / https://discuss.ocaml.org/t/why-wont-ocaml-specialize-weak-type-variables-in-dead-code/7776 *)
 Extraction Inline Show.ShowLevel_of_Show.
-Extraction Inline SolinasReductionReificationCache.reified_solmul_gen.
 
 Inductive int : Set := int_O | int_S (x : int).
 
